ch08/ex01 verifies

chapter08-application-correspondence/solutions/exercise01_solution.dfy
@@ -5,135 +5,247 @@
 
 include "../../chapter07-async-clients/solutions/exercise01_solution.dfy" //#magicinline
 
-// For reference, go see your or the instructors' solution to chapter06-refine/exercises/exercise01.dfy
-module AsyncClientShardedKVProtocol {
+// This module is analogous to the network: it's a trusted module that gets connected to the
+// host protocol via a binding variable. The host says "if the client were to initiate this request,
+// here's how I'd respond;" this module gets to say "whether the client initiated this request".
+// (Just as the network says whether a packet can be received.) This represents the trusted system
+// "observing" requests crossing between the application and the protocol (eg at a library boundary),
+// to ensure that the protocol proof isn't succeeding by simply lying.
+module TrustedABI {
   import opened Library
   import opened Types
 
-  type HostIdx = nat
-
-  datatype Constants = Constants(mapCount: nat)
-  {
-    predicate WF() { 0 < mapCount }
-    predicate ValidHost(idx: HostIdx) { idx < mapCount }
-  }
-
-//#elide TODO(manos): talk around this in the lecture slides. Maybe in a future revision we'd just
-//#elide bite the bullet and throw all the complexity in here, since the students have seen it
-//#elide since chapter 05?
-  // Since the bottom-bread application-visible ABI is a trusted ("player 1")
-  // definition, it should be expressed as part of the DistributedSystem
-  // compound state machine, like the Network module.  We're trying to keep
-  // this exercise simple (atomic Transfers from one host to the next, no
-  // Network), so we'll fake that trusted module split with a dataytpe struct
-  // marked trusted.
-  // "Trusted" here means that player 1 has a way of deciding when this part of
-  // the state should change, for example, requests should only appear when a
-  // client thread actually makes a library downcall.
-  datatype TrustedABI = TrustedABI(requests:set<Input>, replies:set<Output>)
-
-  datatype Variables = Variables(maps:seq<map<Key, Value>>, abi: TrustedABI)
-  {
-    predicate WF(c: Constants) {
-      && c.WF()
-      && |maps| == c.mapCount
-    }
-  }
+  datatype Constants = Constants()  // No constants
+  datatype Variables = Variables(requests:set<Input>, replies:set<Output>)
 
   predicate Init(c: Constants, v: Variables)
   {
-    && v.WF(c)
-    && (forall idx:HostIdx | c.ValidHost(idx) :: v.maps[idx] == if idx==0 then InitialMap() else map[])
-    && v.abi.requests == {}
-    && v.abi.replies == {}
+    && v.requests == {}
+    && v.replies == {}
   }
+
+  // Type of binding variable between Host and TrustedABI. Analogous to Network.MsgOps
+  datatype ABIOps =
+    | ServiceRequestOp(request:Input, reply:Output)
+    | NoOp
+
+  // 
+  // abiOps is a binding variable: protocol says what it'd do if it got that request,
+  // and this module gets to say whether a request is available right now, or record
+  // the fact that the protocol returned a given result.
+  predicate ExecuteOp(c: Constants, v: Variables, v': Variables, abiOps: ABIOps)
+  {
+    match abiOps
+      case ServiceRequestOp(request, reply) =>
+        // Protocol can drop any request it wants, and introduce any reply it
+        // wants; that won't affect meaning, since it ultimately has to get the
+        // incoming requests and outgoing replies to match what the spec
+        // allows.
+        && abiOps.request in v.requests
+        && abiOps.reply !in v.replies
+        && v' == v.(requests := v.requests - {abiOps.request}, replies := v.replies + {abiOps.reply})
+      case NoOp() =>
+        && v' == v
+  }
+
+  // Record the claim that a client actually made this request. This
+  // corresponds to a trusted handler attesting that the client wanted
+  // the request, it wasn't just invented by the protocol.
   predicate AcceptRequest(v:Variables, v':Variables, request: Input)
   {
 //#exercise    false // TODO Define this predicate
 //#start-elide
-    && request !in v.abi.requests // (liveness only) if client picked identical nonces, don't let the requests collapse.
-    && v' == v.(abi := v.abi.(requests := v.abi.requests + {request}))
+    && request !in v.requests
+    && v' == v.(requests := v.requests + {request})
 //#end-elide
   }
 
+  // Record the fact that the client learned this reply. This corresponds
+  // to a trusted handler attesting that this reply was exposed to the
+  // client -- so the spec had better justify the exposed value.
   predicate DeliverReply(v:Variables, v':Variables, reply: Output)
   {
 //#exercise    false // TODO Define this predicate
 //#start-elide
-    && reply in v.abi.replies
-    && v' == v.(abi := v.abi.(replies := v.abi.replies - {reply}))
+    && reply in v.replies
+    && v' == v.(replies := v.replies - {reply})
 //#end-elide
   }
 
-  predicate Insert(c: Constants, v: Variables, v': Variables, idx: HostIdx, request: Input)
+  // JayNF except "Next" is "ClientOp" -- one of two "entry points" to this module.
+  datatype Step =
+    | AcceptRequestStep(request:Input)
+    | DeliverReplyStep(reply: Output)
+
+  predicate ClientOpStep(c:Constants, v:Variables, v':Variables, step: Step)
   {
-    && v.WF(c)
-    && c.ValidHost(idx)
-    && request in v.abi.requests
-    && request.InsertRequest?
-    && var reply := InsertReply(request);
-    && reply !in v.abi.replies
-    && request.key in v.maps[idx] // the participating "host" needs to be authoritative on this key
-    //&& key in AllKeys() // implied by previous conjunct + Inv()ariant
-    && v' == v.(
-      maps := v.maps[idx := v.maps[idx][request.key := request.value]],
-      abi := v.abi.(
-        requests := v.abi.requests - {request},
-        replies := v.abi.replies + {reply}))
-              
+    match step
+      case AcceptRequestStep(request) => AcceptRequest(v, v', request)
+      case DeliverReplyStep(request) => DeliverReply(v, v', request)
   }
 
-  predicate Query(c: Constants, v: Variables, v': Variables, idx: HostIdx, request: Input, output: Value)
+  predicate ClientOp(c:Constants, v:Variables, v':Variables)
   {
-    && v.WF(c)
-    && c.ValidHost(idx)
-    && request in v.abi.requests
-    && request.QueryRequest?
-    && var reply := QueryReply(request, output);
-    && reply !in v.abi.replies
-    && request.key in v.maps[idx] // the participating "host" needs to be authoritative on this key
-    && output == v.maps[idx][request.key]
-    && v' == v.(
-      abi := v.abi.(
-        requests := v.abi.requests - {request},
-        replies := v.abi.replies + {reply}))
+    exists step :: ClientOpStep(c, v, v', step)
+  }
+}
+
+// For reference, go see your or the instructors' solution to chapter06-refine/exercises/exercise01.dfy
+// Note that, in this version, we split up the seq<map> into separate Host state machines (which then
+// there are a seq of in the DistributedSystem), so it feels closer to our canonical compound
+// state machine module of a distributed system. However, to keep this example simple, we still use
+// synchronous communication among hosts (not an asynchronous network).
+module Host {
+  import opened Library
+  import opened Types
+  import TrustedABI
+
+  datatype Constants = Constants(myId: nat) {
+    predicate GroupWF(id: nat) {
+      && myId == id
+    }
   }
 
-  // A possible enhancement exercise: transfer many key,value pairs in one step
-  predicate Transfer(c: Constants, v: Variables, v': Variables, sendIdx: HostIdx, recvIdx: HostIdx, key: Key, value: Value)
+  datatype Variables = Variables(mapp:map<Key, Value>)
+
+  predicate Init(c: Constants, v: Variables)
+  {
+    v.mapp == if c.myId == 0 then InitialMap() else map[]
+  }
+
+  predicate Insert(c: Constants, v: Variables, v': Variables, abiOps: TrustedABI.ABIOps)
+  {
+    && abiOps.ServiceRequestOp?
+    && abiOps.request.InsertRequest?
+    && abiOps.request.key in v.mapp // this host needs to be authoritative on this key
+    && abiOps.reply == InsertReply(abiOps.request)
+    && v' == v.(mapp := v.mapp[abiOps.request.key := abiOps.request.value])
+  }
+
+  predicate Query(c: Constants, v: Variables, v': Variables, abiOps: TrustedABI.ABIOps)
+  {
+    && abiOps.ServiceRequestOp?
+    && abiOps.request.QueryRequest?
+    && abiOps.request.key in v.mapp // this host needs to be authoritative on this key
+    && abiOps.reply.QueryReply?
+    && abiOps.reply.request == abiOps.request
+    && abiOps.reply.output == v.mapp[abiOps.request.key]
+    && v' == v
+  }
+
+  datatype Message = Transfer(key: Key, value: Value)
+
+  // "Entry point" from DistributedSystem: send half of a synchronous message exchange with another host.
+  predicate Send(c: Constants, v: Variables, v': Variables, msg: Message)
+  {
+    && msg.key in v.mapp
+    && v.mapp[msg.key] == msg.value
+    && v' == v.(mapp := MapRemoveOne(v.mapp, msg.key))  // key leaves sending map
+  }
+
+  // "Entry point" from DistributedSystem: receive half of a synchronous message exchange with another host.
+  predicate Recv(c: Constants, v: Variables, v': Variables, msg: Message)
+  {
+    && v' == v.(mapp := v.mapp[msg.key := msg.value])  // key appears in recv map
+  }
+
+  // "Entry point" from DistributedSystem: process a client request that's waiting in the ABI -- a serialization point.
+  predicate Local(c: Constants, v: Variables, v': Variables, abiOps: TrustedABI.ABIOps)
+  {
+    && abiOps.ServiceRequestOp? // We don't have any NoOp Local ops. (Send/Recv is an ABI noop, but it's not Local)
+    && match abiOps.request
+      case InsertRequest(_,_,_) => Insert(c, v, v', abiOps)
+      case QueryRequest(_,_) => Query(c, v, v', abiOps)
+  }
+}
+
+module DistributedSystem {
+  import Host
+  import TrustedABI
+
+  type HostIdx = nat
+
+  datatype Constants = Constants(hosts: seq<Host.Constants>, abi: TrustedABI.Constants)
+  {
+    predicate ValidHost(idx: HostIdx) {
+      idx < |hosts|
+    }
+    predicate WF() {
+      && 0 < |hosts|
+      && (forall idx:HostIdx | ValidHost(idx) :: hosts[idx].GroupWF(idx)) // configure hosts with their id
+    }
+  }
+
+  datatype Variables = Variables(hosts: seq<Host.Variables>, abi: TrustedABI.Variables)
+  {
+    predicate WF(c: Constants) {
+      && c.WF()
+      && |hosts| == |c.hosts|
+    }
+  }
+
+  predicate Init(c:Constants, v:Variables)
+  {
+    && v.WF(c)
+    && (forall idx:HostIdx | c.ValidHost(idx) :: Host.Init(c.hosts[idx], v.hosts[idx]))
+    && TrustedABI.Init(c.abi, v.abi)
+  }
+
+  // ABI records an incoming request or delivers a reply
+  predicate ClientOp(c:Constants, v:Variables, v':Variables)
+  {
+//#exercise    false // TODO Define this predicate
+//#start-elide
+    && v.WF(c)
+    && v'.WF(c)
+    && TrustedABI.ClientOp(c.abi, v.abi, v'.abi)
+    && (forall hostIdx:HostIdx | c.ValidHost(hostIdx) :: v'.hosts[hostIdx] == v.hosts[hostIdx])
+//#end-elide
+  }
+
+  // Because we're cheating with a synchronous network model, this trusted
+  // DistributedSystem model needs to be aware of how the protocol does
+  // transfers (because two hosts are involved) versus other steps (one host at
+  // a time). To keep it simple, we'll disallow interacting with the client
+  // during a communicate step. Just as with the usual Network model, the
+  // protocol (Host module) gets to define its message type.
+  predicate Communicate(c: Constants, v: Variables, v':Variables, sendIdx:HostIdx, recvIdx:HostIdx, msg:Host.Message)
   {
     && v.WF(c)
     && v'.WF(c)
     && c.ValidHost(sendIdx)
     && c.ValidHost(recvIdx)
-    && key in v.maps[sendIdx]
-    && v.maps[sendIdx][key] == value
-    && v' == v.(
-      maps := v.maps[sendIdx := MapRemoveOne(v.maps[sendIdx], key)]  // key leaves sending map
-                    [recvIdx := v.maps[recvIdx][key := value]]       // key appears in recv map
-         // ... no changes to application-visible requests, replies
-      )
+    && Host.Send(c.hosts[sendIdx], v.hosts[sendIdx], v'.hosts[sendIdx], msg)
+    && Host.Recv(c.hosts[recvIdx], v.hosts[recvIdx], v'.hosts[recvIdx], msg)
+    && (forall otherIdx:HostIdx | c.ValidHost(otherIdx) && otherIdx != sendIdx && otherIdx != recvIdx
+          :: v'.hosts[otherIdx] == v.hosts[otherIdx])
+    && v'.abi == v.abi  // UNCHANGED
+  }
+
+  predicate Local(c: Constants, v: Variables, v':Variables, hostIdx:HostIdx, abiOps: TrustedABI.ABIOps)
+  {
+    && v.WF(c)
+    && v'.WF(c)
+    && c.ValidHost(hostIdx)
+    && Host.Local(c.hosts[hostIdx], v.hosts[hostIdx], v'.hosts[hostIdx], abiOps)
+    && (forall otherIdx:HostIdx | c.ValidHost(otherIdx) && otherIdx != hostIdx :: v'.hosts[otherIdx] == v.hosts[otherIdx])
+    && TrustedABI.ExecuteOp(c.abi, v.abi, v'.abi, abiOps)
   }
 
   datatype Step =
-    | AcceptRequestStep(request:Input)
-    | DeliverReplyStep(reply: Output)
-    | InsertStep(idx: HostIdx, request: Input)
-    | QueryStep(idx: HostIdx, request: Input, output: Value)
-    | TransferStep(sendIdx: HostIdx, recvIdx: HostIdx, key: Key, value: Value)
+    | ClientOpStep
+    | CommunicateStep(sendIdx: HostIdx, recvIdx: HostIdx, msg: Host.Message)
+    | LocalStep(hostIdx: HostIdx, abiOps: TrustedABI.ABIOps)
 
-  predicate NextStep(c: Constants, v: Variables, v': Variables, step: Step)
+  predicate NextStep(c: Constants, v: Variables, v':Variables, step: Step)
   {
     match step
-      case AcceptRequestStep(request) => AcceptRequest(v, v', request)
-      case DeliverReplyStep(request) => DeliverReply(v, v', request)
-    
-      case InsertStep(idx, request) => Insert(c, v, v', idx, request)
-      case QueryStep(idx, request, output) => Query(c, v, v', idx, request, output)
-      case TransferStep(sendIdx, recvIdx, key, value) => Transfer(c, v, v', sendIdx, recvIdx, key, value)
+      case ClientOpStep => ClientOp(c, v, v')
+      case CommunicateStep(sendIdx, recvIdx, msg) => Communicate(c, v, v', sendIdx, recvIdx, msg)
+      case LocalStep(hostIdx, abiOps) => Local(c, v, v', hostIdx, abiOps)
   }
 
-  predicate Next(c: Constants, v: Variables, v': Variables)
+  predicate Next(c: Constants, v: Variables, v':Variables)
   {
     exists step :: NextStep(c, v, v', step)
   }
@@ -143,13 +255,13 @@ module RefinementProof {
   import opened Library
   import opened Types
   import MapSpec
-  import opened AsyncClientShardedKVProtocol
+  import opened DistributedSystem
 
   predicate HostHasKey(c: Constants, v: Variables, hostidx:HostIdx, key:Key)
     requires v.WF(c)
   {
     && c.ValidHost(hostidx)
-    && key in v.maps[hostidx]
+    && key in v.hosts[hostidx].mapp
   }
 
   // Pulling the choose out into its own function is sometimes necessary due
@@ -172,7 +284,7 @@ module RefinementProof {
 //#start-elide
     if exists idx :: HostHasKey(c, v, idx, key)
     then
-      v.maps[KeyHolder(c, v, key)][key]
+      v.hosts[KeyHolder(c, v, key)].mapp[key]
     else DefaultValue()
 //#end-elide
   }
@@ -188,7 +300,7 @@ module RefinementProof {
   function MapDomains(c: Constants, v: Variables) : seq<set<Key>>
     requires v.WF(c)
   {
-    seq(c.mapCount, i requires 0<=i<c.mapCount => v.maps[i].Keys)
+    seq(|c.hosts|, i requires 0<=i<|c.hosts| => v.hosts[i].mapp.Keys)
   }
 
   function KnownKeys(c: Constants, v: Variables) : set<Key>
@@ -201,13 +313,13 @@ module RefinementProof {
   // but creates a trigger storm.
   lemma HostKeysSubsetOfKnownKeys(c: Constants, v: Variables, count: nat)
     requires v.WF(c)
-    requires count <= c.mapCount
-    ensures forall idx | 0 <= idx < count :: v.maps[idx].Keys <= KnownKeys(c, v)
+    requires count <= |c.hosts|
+    ensures forall idx | 0 <= idx < count :: v.hosts[idx].mapp.Keys <= KnownKeys(c, v)
   {
-    forall idx | 0 <= idx < count ensures v.maps[idx].Keys <= KnownKeys(c, v)
+    forall idx | 0 <= idx < count ensures v.hosts[idx].mapp.Keys <= KnownKeys(c, v)
     {
       SetsAreSubsetsOfUnion(MapDomains(c, v));
-      assert v.maps[idx].Keys == MapDomains(c, v)[idx];  // trigger
+      assert v.hosts[idx].mapp.Keys == MapDomains(c, v)[idx];  // trigger
     }
   }
 
@@ -233,7 +345,7 @@ module RefinementProof {
   {
     forall key, hostidx:HostIdx, otherhost:HostIdx
         | && c.ValidHost(hostidx) && c.ValidHost(otherhost)
-          && key in v.maps[hostidx] && key in v.maps[otherhost]
+          && key in v.hosts[hostidx].mapp && key in v.hosts[otherhost].mapp
         :: hostidx == otherhost
   }
 
@@ -252,7 +364,7 @@ module RefinementProof {
 //#start-elide
   lemma InitAllKeysEmpty(c: Constants, v: Variables, count: nat)
     requires Init(c, v)
-    requires 0 < count <= c.mapCount
+    requires 0 < count <= |c.hosts|
     ensures KnownKeys(c, v) == AllKeys()
   {
     EachUnionMemberBelongsToASet(MapDomains(c, v));
@@ -270,7 +382,7 @@ module RefinementProof {
     ensures Inv(c, v)
   {
 //#start-elide
-    InitAllKeysEmpty(c, v, c.mapCount);
+    InitAllKeysEmpty(c, v, |c.hosts|);
     reveal_KeysHeldUniquely();
 //#end-elide
   }
@@ -289,24 +401,25 @@ module RefinementProof {
   // This is not a goal by itself, it's one of the cases you'll need to prove
   // NextPreservesInvAndRefines. We've provided its signature to help you
   // structure your overall proof.
-  lemma InsertPreservesInvAndRefines(c: Constants, v: Variables, v': Variables, insertHost: HostIdx, request:Input)
-      returns (specstep: MapSpec.Step)
+  lemma InsertPreservesInvAndRefines(c: Constants, v: Variables, v': Variables, hostIdx: HostIdx, abiOps: TrustedABI.ABIOps)
     requires Inv(c, v)
     requires Next(c, v, v')
-    requires c.ValidHost(insertHost)
-    requires Insert(c, v, v', insertHost, request)
+    requires c.ValidHost(hostIdx)
+    requires Local(c, v, v', hostIdx, abiOps)
+    requires Host.Insert(c.hosts[hostIdx], v.hosts[hostIdx], v'.hosts[hostIdx], abiOps)
     ensures Inv(c, v')
-    ensures MapSpec.NextStep(Abstraction(c, v), Abstraction(c, v'), specstep)
+    ensures MapSpec.NextStep(Abstraction(c, v), Abstraction(c, v'), MapSpec.InsertOpStep(abiOps.request))
   {
 //#start-elide
     var abstractMap := Abstraction(c, v).mapp;
     var abstractMap' := Abstraction(c, v').mapp;
+    var request := abiOps.request;
     var insertedKey := request.key; // use some let-in assignments to recycle chapter06 proof...
     var value := request.value;
 
     assert insertedKey in AllKeys() by {
       SetsAreSubsetsOfUnion(MapDomains(c, v));
-      assert MapDomains(c, v)[insertHost] == v.maps[insertHost].Keys; //trigger
+      assert MapDomains(c, v)[hostIdx] == v.hosts[hostIdx].mapp.Keys; //trigger
     }
 
     assert KeysHeldUniquely(c, v') by { reveal_KeysHeldUniquely(); }
@@ -317,7 +430,7 @@ module RefinementProof {
     {
       if key == insertedKey {
         SetsAreSubsetsOfUnion(MapDomains(c, v'));
-        assert MapDomains(c, v')[insertHost] <= KnownKeys(c, v'); // trigger
+        assert MapDomains(c, v')[hostIdx] <= KnownKeys(c, v'); // trigger
         assert key in abstractMap'; // case goal
       }
       if key in abstractMap {
@@ -331,7 +444,7 @@ module RefinementProof {
       }
       if key in abstractMap' {
         if key == insertedKey {
-          AnyHostWithKeyIsKeyHolder(c, v', insertHost, key);
+          AnyHostWithKeyIsKeyHolder(c, v', hostIdx, key);
           assert abstractMap'[key] == value;  // case goal
         } else {
           var keyIdx := GetIndexForMember(MapDomains(c, v'), key);
@@ -349,7 +462,7 @@ module RefinementProof {
     assert KnownKeys(c, v') == Types.AllKeys() by {
       assert abstractMap'.Keys == KnownKeys(c, v'); // trigger
     }
-    specstep := MapSpec.InsertOpStep(request);  // what used to be a witness is now explicitly exposed.
+    assert MapSpec.NextStep(Abstraction(c, v), Abstraction(c, v'), MapSpec.InsertOpStep(abiOps.request));
 //#end-elide
   }
 
@@ -361,7 +474,7 @@ module RefinementProof {
     EachUnionMemberBelongsToASet(MapDomains(c, v));
 //    assert key in UnionSeqOfSets(MapDomains(c, v));
 //    assert exists idx :: 0<=idx<c.mapCount && key in MapDomains(c, v)[idx];
-    var idx :| 0<=idx<c.mapCount && key in MapDomains(c, v)[idx];
+    var idx :| 0<=idx<|c.hosts| && key in MapDomains(c, v)[idx];
     assert HostHasKey(c, v, idx, key);
   }
 
@@ -382,7 +495,7 @@ module RefinementProof {
   lemma EqualMapsEqualKeysHeldUniquely(c: Constants, v: Variables, v': Variables)
     requires v.WF(c)
     requires v'.WF(c)
-    requires v'.maps == v.maps
+    requires v'.hosts == v.hosts
     ensures KeysHeldUniquely(c, v') == KeysHeldUniquely(c, v)
   {
     reveal_KeysHeldUniquely();
@@ -391,7 +504,7 @@ module RefinementProof {
   lemma EqualMapsEqualMapp(c: Constants, v: Variables, v': Variables)
     requires Inv(c, v)
     requires Inv(c, v')
-    requires v'.maps == v.maps
+    requires v'.hosts == v.hosts
     ensures Abstraction(c, v').mapp == Abstraction(c, v).mapp
   {
     forall k | k in Abstraction(c, v').mapp ensures Abstraction(c, v').mapp[k] == Abstraction(c, v).mapp[k] {
@@ -404,39 +517,42 @@ module RefinementProof {
   // This is not a goal by itself, it's one of the cases you'll need to prove
   // NextPreservesInvAndRefines. We've provided its signature to help you
   // structure your overall proof.
-  lemma QueryPreservesInvAndRefines(c: Constants, v: Variables, v': Variables, queryHost: HostIdx, request: Input, output: Value) returns (specstep: MapSpec.Step)
+  lemma QueryPreservesInvAndRefines(c: Constants, v: Variables, v': Variables, hostIdx: HostIdx, abiOps: TrustedABI.ABIOps)
     requires Inv(c, v)
     requires Next(c, v, v')
-    requires c.ValidHost(queryHost)
-    requires Query(c, v, v', queryHost, request, output)
+    requires c.ValidHost(hostIdx)
+    requires v'.WF(c)
+    requires Local(c, v, v', hostIdx, abiOps)
+    requires Host.Query(c.hosts[hostIdx], v.hosts[hostIdx], v'.hosts[hostIdx], abiOps)
     ensures Inv(c, v')
-    ensures MapSpec.NextStep(Abstraction(c, v), Abstraction(c, v'), specstep)
+    ensures MapSpec.NextStep(Abstraction(c, v), Abstraction(c, v'), MapSpec.QueryOpStep(abiOps.request, abiOps.reply.output))
   {
 //#start-elide
+    var request := abiOps.request;
     var key := request.key;
-    assert v.maps == v'.maps; // weirdly obvious trigger
+    assert v.hosts == v'.hosts; // weirdly obvious trigger
     assert Inv(c, v') by { reveal_KeysHeldUniquely(); }
-    assert key in KnownKeys(c, v) by { HostKeysSubsetOfKnownKeys(c, v, c.mapCount); }
-    assert output == Abstraction(c, v).mapp[key] by {
-      assert HostHasKey(c, v, queryHost, key);  // witness
+    assert key in KnownKeys(c, v) by { HostKeysSubsetOfKnownKeys(c, v, |c.hosts|); }
+    assert abiOps.reply.output == Abstraction(c, v).mapp[key] by {
+      assert HostHasKey(c, v, hostIdx, key);  // witness
       reveal_KeysHeldUniquely();
     }
     EqualMapsEqualMapp(c, v, v');
-    specstep := MapSpec.QueryOpStep(request, output);  // what used to be a witness is now explicitly exposed.
 //#end-elide
   }
 
   // This is not a goal by itself, it's one of the cases you'll need to prove
   // NextPreservesInvAndRefines. We've provided its signature to help you
   // structure your overall proof.
-  lemma TransferPreservesInvAndRefines(c: Constants, v: Variables, v': Variables, sendIdx: HostIdx, recvIdx: HostIdx, sentKey: Key, value: Value) returns (specstep: MapSpec.Step)
+  lemma TransferPreservesInvAndRefines(c: Constants, v: Variables, v': Variables, sendIdx: HostIdx, recvIdx: HostIdx, msg:Host.Message)
     requires Inv(c, v)
     requires Next(c, v, v')
     requires c.ValidHost(sendIdx)
     requires c.ValidHost(recvIdx)
-    requires Transfer(c, v, v', sendIdx, recvIdx, sentKey, value)
+    requires Host.Send(c.hosts[sendIdx], v.hosts[sendIdx], v'.hosts[sendIdx], msg)
+    requires Host.Recv(c.hosts[recvIdx], v.hosts[recvIdx], v'.hosts[recvIdx], msg)
     ensures Inv(c, v')
-    ensures MapSpec.NextStep(Abstraction(c, v), Abstraction(c, v'), specstep)
+    ensures MapSpec.NextStep(Abstraction(c, v), Abstraction(c, v'), MapSpec.NoOpStep)
   {
 //#start-elide
     // domain preserved
@@ -446,7 +562,7 @@ module RefinementProof {
       var idx;
       if key in Abstraction(c, v).mapp {
         SetsAreSubsetsOfUnion(MapDomains(c, v'));
-        if key==sentKey {
+        if key==msg.key {
           idx := recvIdx;
         }
         else {
@@ -457,7 +573,7 @@ module RefinementProof {
       }
       if key in Abstraction(c, v').mapp {
         SetsAreSubsetsOfUnion(MapDomains(c, v));
-        if key==sentKey {
+        if key==msg.key {
           idx := sendIdx;
         }
         else {
@@ -476,7 +592,7 @@ module RefinementProof {
     {
       // identify where to find key in the old & new worlds
       var idx, idx';
-      if key == sentKey {
+      if key == msg.key {
         idx := sendIdx;
         idx' := recvIdx;
       } else {
@@ -494,25 +610,21 @@ module RefinementProof {
       assert KnownKeys(c, v') == Abstraction(c, v').mapp.Keys;  // trigger
       assert KnownKeys(c, v) == Abstraction(c, v).mapp.Keys;    // trigger
     }
-    specstep := MapSpec.NoOpStep; // what used to be a witness is now explicitly exposed.
 //#end-elide
   }
 
-  // This trusted predicate forces application-visible actions to keep the same labels.
-  predicate RefinementHonorsApplicationCorrespondence(c: Constants, v: Variables, v': Variables, step: Step)
+  // Player 2 can define any Abstraction function they want, but it must
+  // synchronize the application-visible requests and replies from the
+  // protocol-level ABI to the spec-level model.
+  lemma RefinementHonorsApplicationCorrespondence(c: Constants, v: Variables)
     requires Inv(c, v)
-    requires NextStep(c, v, v', step)
+    // It's wonky that we have to look inside the untrusted 'v' to find the abi state,
+    // but that's a consequence of the wonky choice of tucking the trusted ABI into the
+    // protocol module, rather than having a trusted DistributedSystem that contains
+    // the untrusted host protocol module; see comments above.
+    ensures Abstraction(c, v).requests == v.abi.requests
+    ensures Abstraction(c, v).replies == v.abi.replies
   {
-    // Application-visible steps are labeled as such in the spec action
-    && (step.AcceptRequestStep?
-        ==> MapSpec.NextStep(Abstraction(c, v), Abstraction(c, v'), MapSpec.AcceptRequestStep(step.request)))
-    && (step.DeliverReplyStep?
-        ==> MapSpec.NextStep(Abstraction(c, v), Abstraction(c, v'), MapSpec.DeliverReplyStep(step.reply)))
-    // If protocol step isn't application-visible...
-    && (!step.AcceptRequestStep? && !step.DeliverReplyStep? ==>
-        // then whatever happened in the spec wasn't an application-visible step.
-        forall specstep:MapSpec.Step | specstep.AcceptRequestStep? || specstep.DeliverReplyStep?
-          :: !MapSpec.NextStep(Abstraction(c, v), Abstraction(c, v'), specstep))
   }
 
   // The proof goal is modified from chapter06 to expose the protocl- and
@@ -520,36 +632,42 @@ module RefinementProof {
   // as an ensures. So where we used to just producte a witness to the application-level
   // step, we now have to actually return it to satisfy the lemmas' mentions of NextStep
   // (instead of just Next).
-  lemma RefinementNext(c: Constants, v: Variables, v': Variables, step: Step) returns (specstep: MapSpec.Step)
+  lemma RefinementNext(c: Constants, v: Variables, v': Variables, step: Step)
     requires Inv(c, v)
     requires NextStep(c, v, v', step)
     ensures Inv(c, v')
-    ensures MapSpec.NextStep(Abstraction(c, v), Abstraction(c, v'), specstep)
-    ensures RefinementHonorsApplicationCorrespondence(c, v, v', step) // demand proof of application correspondence
+    ensures MapSpec.Next(Abstraction(c, v), Abstraction(c, v'))
   {
     // Use InsertPreservesInvAndRefines, QueryPreservesInvAndRefines, and
     // TransferPreservesInvAndRefines here to complete this proof.
 //#start-elide
+    var av := Abstraction(c, v);
+    var av' := Abstraction(c, v');
     var step :| NextStep(c, v, v', step);
     match step
-      case AcceptRequestStep(request) => {
+      case ClientOpStep => {
         EqualMapsEqualKeysHeldUniquely(c, v, v');
         EqualMapsEqualMapp(c, v, v');
-        specstep := MapSpec.AcceptRequestStep(request);
+        var abistep :| TrustedABI.ClientOpStep(c.abi, v.abi, v'.abi, abistep);
+        match abistep
+          case AcceptRequestStep(request) => {
+            assert MapSpec.NextStep(av, av', MapSpec.AcceptRequestStep(request)); // witness step
+          }
+          case DeliverReplyStep(request) => {
+            assert MapSpec.NextStep(av, av', MapSpec.DeliverReplyStep(request)); // witness step
+          }
       }
-      case DeliverReplyStep(request) => {
-        EqualMapsEqualKeysHeldUniquely(c, v, v');
-        EqualMapsEqualMapp(c, v, v');
-        specstep := MapSpec.DeliverReplyStep(request);
+      case CommunicateStep(sendIdx, recvIdx, msg) => {
+        TransferPreservesInvAndRefines(c, v, v', sendIdx, recvIdx, msg);
       }
-      case InsertStep(idx, request) => {
-        specstep := InsertPreservesInvAndRefines(c, v, v', idx, request);
-      }
-      case QueryStep(idx, request, output) => {
-        specstep := QueryPreservesInvAndRefines(c, v, v', idx, request, output);
-      }
-      case TransferStep(sendIdx, recvIdx, key, value) => {
-        specstep := TransferPreservesInvAndRefines(c, v, v', sendIdx, recvIdx, key, value);
+      case LocalStep(hostIdx, abiOps) => {
+        match abiOps.request
+          case InsertRequest(_,_,_) => {
+            InsertPreservesInvAndRefines(c, v, v', hostIdx, abiOps);
+          }
+          case QueryRequest(_,_) => {
+            QueryPreservesInvAndRefines(c, v, v', hostIdx, abiOps);
+          }
       }
 //#end-elide
   }
